Patch up transitivity. Get Ewhile implemented

src/named/CompilerTransitivity.v
@@ -6,7 +6,7 @@ Import ListNotations.
 Open Scope string.
 Open Scope list.
 From Utils Require Import Utils.
-From Named Require Import Core Compilers.
+From Named Require Import Core Compilers ModelImpls.
 Import Core.Notations.
 (*TODO: repackage this in compilers*)
 Import CompilerDefs.Notations.
@@ -25,27 +25,28 @@ Section WithVar.
   Notation subst := (@subst V).
   Notation rule := (@rule V).
   Notation lang := (@lang V).
-  Notation compiler_case := (@compiler_case V).
-  Notation compiler := (@compiler V).
-  Notation compile := (@compile V).
-  Notation compile_subst := (@compile_subst V).
-  Notation compile_ctx := (@compile_ctx V).
-  Notation compile_sort := (@compile_sort V).
+  Notation compiler_case := (compiler_case V (tgt_term:=term) (tgt_sort:=sort)).
+  Notation compiler := (compiler V (tgt_term:=term) (tgt_sort:=sort)).
+  Notation compile l := (compile (V:=V) (tgt_term:=term) (tgt_sort:=sort) (tgt_Model:=core_model l)).
+  Notation compile_subst l := (compile_subst (V:=V) (tgt_term:=term) (tgt_sort:=sort) (tgt_Model:=core_model l)).
+  Notation compile_ctx l := (compile_ctx (V:=V) (tgt_term:=term) (tgt_sort:=sort) (tgt_Model:=core_model l)).
+  Notation compile_args l := (compile_args (V:=V) (tgt_term:=term) (tgt_sort:=sort) (tgt_Model:=core_model l)).
+  Notation compile_sort l := (compile_sort (V:=V) (tgt_term:=term) (tgt_sort:=sort) (tgt_Model:=core_model l)).
   
-
-Lemma compile_subst_combine cmp args s
-  : compile_subst cmp (combine args s) = combine args (map (compile cmp) s).
+Lemma compile_subst_combine l (cmp : compiler) args s
+  : compile_subst l cmp (combine args s) = combine args (map (compile l cmp) s).
 Proof.
   revert args; induction s; destruct args; basic_goal_prep; basic_core_crush.
 Qed.
 
 Section CompileFn.
+  Context (tgt : lang).
   Context (cmp : compiler).
 
   Definition compile_ccase (c : compiler_case) :=
     match c with
-    | sort_case args t => sort_case args (compile_sort cmp t)
-    | term_case args e => term_case args (compile cmp e)
+    | sort_case args t => sort_case args (compile_sort tgt cmp t)
+    | term_case args e => term_case args (compile tgt cmp e)
     end.
 
   Definition compile_cmp (c: compiler) := named_map compile_ccase c.
@@ -108,7 +109,7 @@ Qed.
 Hint Rewrite named_map_combine : utils.
 
 (*TODO: move to Compilers.v*)
-Definition ws_ccase cc :=
+Definition ws_ccase (cc : compiler_case) :=
   match cc with
   | term_case args e => well_scoped args e
   | sort_case args e => well_scoped args e
@@ -136,12 +137,12 @@ Qed.
   might help with inductive_implies_semantic last induction?
  *)
 
-Lemma compile_term_subst cmp e s
+Lemma compile_term_subst l (cmp : compiler) e s
   : all_fresh cmp ->
     all ws_ccase (map snd cmp) ->
     term_in_cmp_domain cmp e ->
     well_scoped (map fst s) e ->
-    compile cmp e[/s/] = (compile cmp e)[/compile_subst cmp s/].
+    compile l cmp e[/s/] = (compile l cmp e)[/compile_subst l cmp s/].
 Proof.
   intros allfcmp all_ws.
   induction e; basic_goal_prep; basic_core_firstorder_crush.
@@ -150,40 +151,43 @@ Proof.
   pose proof (in_all_fresh_same _ _ _ _ allfcmp H0 HeqH4).
   subst.
 
-  rewrite subst_assoc.
+  erewrite subst_assoc.
+  2: typeclasses eauto.
   2:{
-    basic_core_firstorder_crush.
+    rewrite map_fst_combine_r_padded.
     eapply in_ws_term_cmp; eauto.
   }
   f_equal.
   unfold subst_cmp.
-  basic_utils_crush.
+  rewrite named_map_combine_r_padded; [|reflexivity].
   f_equal.
 
   (*prove inner induction*)
   clear x x0 H0 H2 HeqH4.
-  revert dependent l.
-  induction l; basic_goal_prep; basic_core_crush.
+  revert dependent l0.
+  induction l0; basic_goal_prep; basic_core_crush.
 Qed.
 Hint Rewrite compile_term_subst : lang_core.
 
 
-Lemma compile_args_subst cmp e s
+Lemma compile_args_subst l cmp e s
   : all_fresh cmp ->
     all ws_ccase (map snd cmp) ->
     all (term_in_cmp_domain cmp) e ->
     well_scoped (map fst s) e ->
-    compile_args cmp e[/s/] = (compile_args cmp e)[/compile_subst cmp s/].
+    compile_args l cmp e[/s/] = (compile_args l cmp e)[/compile_subst l cmp s/].
 Proof.
   induction e; basic_goal_prep; basic_core_crush.
+  fold_Substable.
+  basic_core_crush.
 Qed.
 
-Lemma compile_sort_subst cmp e s
+Lemma compile_sort_subst l cmp e s
   : all_fresh cmp ->
     all ws_ccase (map snd cmp) ->
     sort_in_cmp_domain cmp e ->
     well_scoped (map fst s) e ->
-    compile_sort cmp e[/s/] = (compile_sort cmp e)[/compile_subst cmp s/].
+    compile_sort l cmp e[/s/] = (compile_sort l cmp e)[/compile_subst l cmp s/].
 Proof.
   intros allfcmp all_ws.
   induction e; basic_goal_prep; basic_core_firstorder_crush.
@@ -192,20 +196,21 @@ Proof.
   pose proof (in_all_fresh_same _ _ _ _ allfcmp H HeqH3).
   subst.
 
-  rewrite subst_assoc.
+  erewrite subst_assoc; try typeclasses eauto.
   2:{
-    basic_core_firstorder_crush.
+    rewrite map_fst_combine_r_padded.
     eapply in_ws_sort_cmp; eauto.
   }
   f_equal.
   unfold subst_cmp.
-  basic_utils_crush.
+  rewrite named_map_combine_r_padded.
   f_equal.
   apply compile_args_subst; eauto.
+  reflexivity.
 Qed.
 Hint Rewrite compile_sort_subst : lang_core.
 
-Definition ccase_in_cmp_domain cmp cc :=
+Definition ccase_in_cmp_domain (cmp : compiler) (cc : compiler_case) :=
   match cc with
   | term_case _ e => term_in_cmp_domain cmp e
   | sort_case _ e => sort_in_cmp_domain cmp e
@@ -219,15 +224,19 @@ Proof.
 Qed.
 Hint Resolve pair_in_map_snd : utils.
 
-Lemma compile_cmp_distributes cmp cmp' e
-  : all ws_ccase (map snd cmp) ->
+
+Lemma compile_cmp_distributes tgt ir cmp cmp' e
+  : 
+  (*TODO: find a better way to discharge this*)
+  compile tgt cmp default = default ->
+  all ws_ccase (map snd cmp) ->
     all_fresh cmp ->
     all ws_ccase (map snd cmp') ->
     all_fresh cmp' ->
     all (ccase_in_cmp_domain cmp) (map snd cmp') ->
     term_in_cmp_domain cmp' e ->
-    (compile (compile_cmp cmp cmp') e)
-    = (compile cmp (compile cmp' e)).
+    (compile tgt (compile_cmp tgt cmp cmp') e)
+    = (compile tgt cmp (compile ir cmp' e)).
 Proof.
   intros all_ws_cmp allfr_cmp all_ws_cmp' allfr_cmp' cmp'_in_dom.
   induction e; basic_goal_prep; basic_core_firstorder_crush.
@@ -235,30 +244,31 @@ Proof.
   {
     rewrite all_fresh_named_list_lookup_err_in; eauto.
   }
-  rewrite <- H3.
-  assert (Some (term_case x (compile cmp x0))
-          = named_list_lookup_err (compile_cmp cmp cmp') n).
+  rewrite <- H4.
+  assert (Some (term_case x (compile tgt cmp x0))
+          = named_list_lookup_err (compile_cmp tgt cmp cmp') n).
   {
     rewrite all_fresh_named_list_lookup_err_in.
     2: unfold compile_cmp; basic_utils_crush.
-    rewrite all_fresh_named_list_lookup_err_in in H3; eauto.
+    rewrite all_fresh_named_list_lookup_err_in in H4; eauto.
     unfold compile_cmp.
-    change (term_case x (compile cmp x0))
-      with (compile_ccase cmp (term_case x x0)).
+    change (term_case x (compile tgt cmp x0))
+      with (compile_ccase tgt cmp (term_case x x0)).
     eapply in_named_map; eauto.
   }
-  rewrite <- H4.
+  rewrite <- H5.
   erewrite compile_term_subst; unfold ws_lang;eauto.
 
   {
     f_equal.
     unfold compile_subst.
     autorewrite with utils.
+    rewrite named_map_combine_r_padded; auto.
     f_equal.
     
 
     (*nested induction*)
-    clear x x0 H0 H1 H3 H4.
+    clear x x0 H1 H2 H4 H5.
     revert dependent l.
     induction l; basic_goal_prep; basic_core_crush.
   }
@@ -270,37 +280,44 @@ Proof.
     }
     repeat autorewrite with utils; auto.
   }
-  repeat autorewrite with utils; auto.
+  rewrite map_fst_combine_r_padded.
   eapply in_ws_term_cmp; [|eauto]; eauto.
+  
 Qed.
 Hint Rewrite compile_cmp_distributes : lang_core.
 
 
-Lemma compile_args_cmp_distributes cmp cmp' e
-  : all ws_ccase (map snd cmp) ->
+Lemma compile_args_cmp_distributes tgt ir cmp cmp' e
+  :  (*TODO: find a better way to discharge this*)
+  compile tgt cmp default = default ->
+  all ws_ccase (map snd cmp) ->
     all_fresh cmp ->
     all ws_ccase (map snd cmp') ->
     all_fresh cmp' ->
     all (ccase_in_cmp_domain cmp) (map snd cmp') ->
     all (term_in_cmp_domain cmp') e ->
-    (compile_args (compile_cmp cmp cmp') e)
-    = (compile_args cmp (compile_args cmp' e)).
+    (compile_args tgt (compile_cmp tgt cmp cmp') e)
+    = (compile_args tgt cmp (compile_args ir cmp' e)).
 Proof.
   intros all_ws_cmp allfr_cmp all_ws_cmp' allfr_cmp' cmp'_in_dom.
   induction e; basic_goal_prep; basic_core_crush.
+
+  eapply compile_cmp_distributes; eauto.
 Qed.
 Hint Rewrite compile_args_cmp_distributes : lang_core.
 
 
-Lemma compile_sort_cmp_distributes cmp cmp' e
-  : all ws_ccase (map snd cmp) ->
+Lemma compile_sort_cmp_distributes tgt ir cmp cmp' e
+  :   (*TODO: find a better way to discharge this*)
+  compile tgt cmp default = default ->
+  all ws_ccase (map snd cmp) ->
     all_fresh cmp ->
     all ws_ccase (map snd cmp') ->
     all_fresh cmp' ->
     all (ccase_in_cmp_domain cmp) (map snd cmp') ->
     sort_in_cmp_domain cmp' e ->
-    (compile_sort (compile_cmp cmp cmp') e)
-    = (compile_sort cmp (compile_sort cmp' e)).
+    (compile_sort tgt (compile_cmp tgt cmp cmp') e)
+    = (compile_sort tgt cmp (compile_sort ir cmp' e)).
 Proof.
   intros all_ws_cmp allfr_cmp all_ws_cmp' allfr_cmp' cmp'_in_dom.
   destruct e; basic_goal_prep; basic_core_firstorder_crush.
@@ -308,32 +325,35 @@ Proof.
   {
     rewrite all_fresh_named_list_lookup_err_in; eauto.
   }
-  rewrite <- H2.
-  assert (Some (sort_case x (compile_sort cmp x0))
-          = named_list_lookup_err (compile_cmp cmp cmp') v).
+  rewrite <- H3.
+  assert (Some (sort_case x (compile_sort tgt cmp x0))
+          = named_list_lookup_err (compile_cmp tgt cmp cmp') v).
   {
     rewrite all_fresh_named_list_lookup_err_in.
     2: unfold compile_cmp; basic_utils_crush.
-    rewrite all_fresh_named_list_lookup_err_in in H2; eauto.
+    rewrite all_fresh_named_list_lookup_err_in in H3; eauto.
     unfold compile_cmp.
-    change (sort_case x (compile_sort cmp x0))
-      with (compile_ccase cmp (sort_case x x0)).
+    change (sort_case x (compile_sort tgt cmp x0))
+      with (compile_ccase tgt cmp (sort_case x x0)).
     eapply in_named_map; eauto.
   }
-  rewrite <- H3.
+  rewrite <- H4.
   erewrite compile_sort_subst; unfold ws_lang;eauto.
 
   {
     f_equal.
     unfold compile_subst.
-    autorewrite with utils.
+    rewrite named_map_combine_r_padded.
     f_equal.
     
 
     (*nested induction*)
-    clear x x0 H0 H H2 H3.
+    clear x x0 H1 H0 H3 H4.
     revert dependent l.
     induction l; basic_goal_prep; basic_core_crush.
+    all: auto.
+    
+    eapply compile_cmp_distributes; eauto.
   }
   {
     assert  (ccase_in_cmp_domain cmp (sort_case x x0)).
@@ -343,35 +363,40 @@ Proof.
     }
     repeat autorewrite with utils; auto.
   }
+  rewrite map_fst_combine_r_padded.
   repeat autorewrite with utils; auto.
   eapply in_ws_sort_cmp; [|eauto]; eauto.
 Qed.
 Hint Rewrite compile_sort_cmp_distributes : lang_core.
 
 
-Lemma compile_ctx_cmp_distributes cmp cmp' e
-  : all ws_ccase (map snd cmp) ->
+Lemma compile_ctx_cmp_distributes tgt ir cmp cmp' e
+  :   (*TODO: find a better way to discharge this*)
+  compile tgt cmp default = default ->
+  all ws_ccase (map snd cmp) ->
     all_fresh cmp ->
     all ws_ccase (map snd cmp') ->
     all_fresh cmp' ->
     all (ccase_in_cmp_domain cmp) (map snd cmp') ->
     all (sort_in_cmp_domain cmp') (map snd e) ->
-    (compile_ctx (compile_cmp cmp cmp') e)
-    = (compile_ctx cmp (compile_ctx cmp' e)).
+    (compile_ctx tgt (compile_cmp tgt cmp cmp') e)
+    = (compile_ctx tgt cmp (compile_ctx ir cmp' e)).
 Proof.
   intros all_ws_cmp allfr_cmp all_ws_cmp' allfr_cmp' cmp'_in_dom.
   induction e; basic_goal_prep; basic_core_crush.
+  erewrite compile_sort_cmp_distributes; eauto.
+  erewrite H3; eauto.
 Qed.
 Hint Rewrite compile_ctx_cmp_distributes : lang_core.   
 
 
 Lemma preserving_is_well_scoped cmp_pre tgt cmp ir
   : ws_lang tgt ->
-    preserving_compiler_ext cmp_pre tgt cmp ir ->
+    preserving_compiler_ext (tgt_Model:=core_model tgt) cmp_pre cmp ir ->
     all ws_ccase (map snd cmp).
 Proof.
   induction 2; basic_goal_prep; intuition;
-    replace (map fst c) with (map fst (compile_ctx (cmp++cmp_pre) c)).
+    replace (map fst c) with (map fst (compile_ctx tgt (cmp++cmp_pre) c)).
   eapply wf_sort_implies_ws; eauto.
   apply named_map_fst_eq; eauto.
   eapply wf_term_implies_ws; eauto.
@@ -381,7 +406,7 @@ Hint Resolve preserving_is_well_scoped : lang_core.
 
 
 Lemma sort_in_preserving_lang_in_cmp cmp_pre tgt cmp src n c' args
-  : preserving_compiler_ext cmp_pre tgt cmp src ->
+  : preserving_compiler_ext (tgt_Model:=core_model tgt) cmp_pre cmp src ->
     In (n, sort_rule c' args) src ->
     exists t, In (n, sort_case (map fst c') t) cmp.
 Proof.
@@ -390,7 +415,7 @@ Proof.
 Qed.
 
 Lemma term_in_preserving_lang_in_cmp cmp_pre tgt cmp src n c' args t
-  : preserving_compiler_ext cmp_pre tgt cmp src ->
+  : preserving_compiler_ext (tgt_Model:=core_model tgt) cmp_pre cmp src ->
     In (n, term_rule c' args t) src ->
     exists e, In (n, term_case (map fst c') e) cmp.
 Proof.
@@ -401,7 +426,7 @@ Qed.
 
 
 Lemma wf_in_domain cmp_pre tgt cmp src
-  : preserving_compiler_ext cmp_pre tgt cmp src ->    
+  : preserving_compiler_ext (tgt_Model:=core_model tgt) cmp_pre cmp src ->    
     (forall c t,
         wf_sort src c t ->
         sort_in_cmp_domain cmp t)
@@ -409,7 +434,7 @@ Lemma wf_in_domain cmp_pre tgt cmp src
            wf_term src c e t ->
            term_in_cmp_domain cmp e)
     /\ (forall c s' c',
-           wf_args src c s' c' ->
+           wf_args (Model:=core_model src) c s' c' ->
            all (term_in_cmp_domain cmp) s').
 Proof.
   intro pres_cmp.
@@ -433,7 +458,7 @@ Qed.
 
   
 Lemma wf_term_in_domain cmp_pre tgt cmp ir c e t
-  : preserving_compiler_ext cmp_pre tgt cmp ir ->
+  : preserving_compiler_ext (tgt_Model:=core_model tgt) cmp_pre cmp ir ->
     wf_term ir c e t ->
     term_in_cmp_domain cmp e.
 Proof.
@@ -442,7 +467,7 @@ Qed.
 Hint Resolve wf_term_in_domain : lang_core.
 
 Lemma wf_sort_in_domain cmp_pre tgt cmp ir c t
-  : preserving_compiler_ext cmp_pre tgt cmp ir ->
+  : preserving_compiler_ext (tgt_Model:=core_model tgt) cmp_pre cmp ir ->
     wf_sort ir c t ->
     sort_in_cmp_domain cmp t.
 Proof.
@@ -451,8 +476,8 @@ Qed.
 Hint Resolve wf_sort_in_domain : lang_core.
 
 Lemma wf_ctx_in_domain cmp_pre tgt cmp ir c
-  : preserving_compiler_ext cmp_pre tgt cmp ir ->
-    wf_ctx ir c ->
+  : preserving_compiler_ext (tgt_Model:=core_model tgt) cmp_pre cmp ir ->
+    wf_ctx (Model:= core_model ir) c ->
     all (sort_in_cmp_domain cmp) (map snd c).
 Proof.
   induction 2; basic_goal_prep; basic_core_crush.
@@ -460,8 +485,8 @@ Qed.
 Hint Resolve wf_ctx_in_domain : lang_core.
   
 Lemma preserving_in_domain cmp_pre tgt cmp ir cmp' src
-  : preserving_compiler_ext cmp_pre tgt cmp ir ->
-    preserving_compiler_ext [] ir cmp' src ->
+  : preserving_compiler_ext (tgt_Model:=core_model tgt) cmp_pre cmp ir ->
+    preserving_compiler_ext (tgt_Model:=core_model ir ) [] cmp' src ->
     all (ccase_in_cmp_domain cmp) (map snd cmp').
 Proof.
   intro pres_cmp.
@@ -470,26 +495,91 @@ Proof.
   eapply wf_term_in_domain; eauto.
 Qed.
 Hint Resolve preserving_in_domain : lang_core.
+
+
+Lemma compiler_map_fst_incl tgt cmp l
+  : preserving_compiler_ext (tgt_Model:=core_model tgt) [] cmp l ->
+    incl (map fst cmp) (map fst l).
+Proof.
+  induction 1;
+    basic_goal_prep;
+    basic_core_crush.
+Qed.
+
+(*
+Lemma all_fresh_incl {A B} (cmp : @Utils.named_list V A) (l : @Utils.named_list V B)
+  : incl (map fst cmp) (map fst l) ->
+    all_fresh l ->
+    all_fresh cmp.
+Proof.
+  revert cmp.
+  induction l;
+    basic_goal_prep;
+    basic_core_crush.
+  {
+    destruct cmp; simpl in *; auto.
+    inversion H.
+  }
+  {
+    eapply IHl; auto.
+  }
+  all_fresh_conflict_impossible
+    all_fresh_in_once
+Qed.*)
+
+Lemma all_fresh_compiler tgt cmp l
+  : preserving_compiler_ext (tgt_Model:=core_model tgt) [] cmp l ->
+    all_fresh l ->
+    all_fresh cmp.
+Proof.
+  induction 1;
+    basic_goal_prep;
+    basic_core_crush.
+  {
+    unfold fresh in *.
+    intro; apply H2.
+    eapply compiler_map_fst_incl; eauto.
+  }
+  {
+    unfold fresh in *.
+    intro; apply H2.
+    eapply compiler_map_fst_incl; eauto.
+  }
+Qed.
+Hint Resolve all_fresh_compiler : lang_core.
   
 (*TODO: can cmp be generalized w/ a cmp_pre?*)
 Theorem preservation_transitivity src ir tgt cmp cmp'
-  : wf_lang src ->
+  :  (*TODO: find a better way to discharge this*)
+  compile tgt cmp default = default ->
+ wf_lang src ->
     wf_lang ir ->
     wf_lang tgt ->
-    preserving_compiler_ext [] tgt cmp ir ->
-    preserving_compiler_ext [] ir cmp' src ->
-    preserving_compiler_ext [] tgt (compile_cmp cmp cmp') src.
+    (forall s : @Substable.subst V (Term.term V),
+  @eq (Term.sort V)
+    (@apply_subst V (Term.term V) (Term.sort V) (@sort_substable V (Term.term V) (Term.sort V) (core_model tgt)) s
+       (default)) (default)) ->
+    (forall s : @Substable.subst V (Term.term V),
+  @eq (Term.term V)
+    (@apply_subst0 V (Term.term V) (@term_substable V (Term.term V) (Term.sort V) (core_model tgt)) s
+       (default)) (default)) ->
+    preserving_compiler_ext (tgt_Model:=core_model tgt) [] cmp ir ->
+    preserving_compiler_ext (tgt_Model:=core_model ir) [] cmp' src ->
+    preserving_compiler_ext (tgt_Model:=core_model tgt) [] (compile_cmp tgt cmp cmp') src.
 Proof using .
-  intros wfsrc wfir wftgt pres_cmp pres_cmp'.
-  pose proof (inductive_implies_semantic wfir wftgt pres_cmp).
+  intros  compile_default wfsrc wfir wftgt sub_default sub_default' pres_cmp pres_cmp'.
+  pose proof (inductive_implies_semantic (tgt_Model_ok := core_model_ok wftgt)
+                sub_default sub_default' wfir pres_cmp).
   firstorder.
   revert wfsrc.
   induction pres_cmp'; basic_goal_prep; constructor;
     autorewrite with lang_core utils in *; firstorder eauto.
-  1,8,21,40:solve [apply inductive_implies_semantic in pres_cmp'; firstorder].
+  all:  erewrite ?compile_ctx_cmp_distributes, ?compile_sort_cmp_distributes, ?compile_cmp_distributes.
   all: eauto with lang_core.
-  all: try match goal with [|- all_fresh _] => basic_core_crush end.
-  all: basic_core_firstorder_crush.
+  all: pose proof (core_model_ok wfir).
+  all:solve [apply inductive_implies_semantic in pres_cmp'; firstorder; constructor].
+  Unshelve.
+  all: exact tgt.
 Qed.
 Hint Resolve preservation_transitivity : lang_core.
 
